\documentclass[../main]{subfiles}

\pgfplotsset{every axis/.append style={
                    axis x line=middle,    % put the x axis in the middle
                    axis y line=middle,    % put the y axis in the middle
                    axis line style={<->}, % arrows on the axis
                    xlabel={$x$},          % default put x on x-axis
                    ylabel={$y$},          % default put y on y-axis
                    }}
\tikzset{>=stealth}

\begin{document}

\section{Assumed Knowledge}

\subsection{Algebra}

	\subsubsection{Completing the Square}
	\[ x^2+bx+c = (x+\frac{b}{2})^2+c-(\frac{b}{2})^2 \]
	\subsubsection{Polynomial Expansions}
	\begin{equation*} \begin{gathered}
		(a\pm b)^2 = a^2 \pm 2ab + b^2 \\
		a^2 - b^2 = (a+b)(a-b) \\
		a^3 \pm b^3 = (a \pm b)(a^2 \mp 2ab + b^2)
	\end{gathered} \end{equation*}
	\subsubsection{Partal Fractions}
	\begin{equation*} \begin{gathered}
		\frac{f(x)}{(ax+b)(cx+d)} \\ = g(x) + \frac{A}{ax+b} + \frac{B}{cx+d} \\
		\frac{f(x)}{(ax+b)(cx+d)^2} \\ = g(x) + \frac{A}{ax+b} + \frac{B}{cx+d} + \frac{C}{(cx+d)^2} \\
		\frac{f(x)}{(ax+b)(x^2+c)} \\ = g(x) + \frac{A}{ax+b} + \frac{Bx+C}{x^2+c}
	\end{gathered} \end{equation*}
	\subsubsection{Exponent and Logarithm}
	\begin{equation*} \begin{gathered}
		e^n = \underbrace{e \times e \times e \times ... \times e}_\text{n times} \\
		e^\frac{1}{2} = \sqrt{e} \\
		log_{e}(x) = ln(x) \\ = \text{how many times \(e\) is multiplied by itself to get x} \\
		log_{10}(x) = lg(x) \\
		x = e^{ln(x)} \\
		log_x(y) = \frac{log_{base}(y)}{log_{base}(x)} 
	\end{gathered} \end{equation*}
	\begin{tikzpicture} \begin{axis}[domain=-5:5,ymin=-5,ymax=5,samples=100,mark=none,smooth]
	    \addplot[color=black,no marks,line width=1pt,-] {e^x} node[pos=0.03,anchor=south east]{$e^x$};
	    \addplot[color=black,no marks,line width=1pt,-] {ln(x)} node[pos=0.75,anchor=south east]{$ln(x)$};  
	\end{axis} \end{tikzpicture}

\subsection{Trigonometry}
	
	\subsubsection{Sine and Cosine Rule}
	For any triangle with length of sides \(a\), \(b\) and \(c\) and with opposite angles \(A\) \(B\) and \(C\):
	\begin{equation*} \begin{gathered}
		\frac{a}{sin(A)}=\frac{b}{sin(B)}=\frac{c}{sin(C)} \\
		a^2 = b^2 + c^2 - 2 b c cos(A) \\
		cos(A) = \frac{b^2 + c^2 - a^2}{2bc}
	\end{gathered} \end{equation*}
	\subsubsection{Sum of Angles}
	\begin{equation*} \begin{gathered}
		sin(A \pm B) = sin(A)cos(B) \pm cos(A)sin(B) \\
		sin(2A) = 2sin(A)cos(A) \\
		cos(A \pm B) = cos(A)cos(B) \mp sin(A)sin(B) \\
	\end{gathered} \end{equation*}
	\begin{equation*} \begin{split}
		cos(2A) & = cos^2(A) - sin^2(A) \\
				& = 2cos^2(A) - 1 \\
				& = 1 - 2sin^2(A)
	\end{split} \end{equation*}
	\begin{equation*} \begin{gathered}
		tan(A \pm B) = \frac{tan(A) \pm tan(B)}{1 \mp tan(A)tan(B)} \\
		tan(2A) = \frac{2tan(A)}{1-tan^2(A)} 
	\end{gathered} \end{equation*}
	\[ \text{Area of Triangle} = \tfrac{1}{2}absin(C) \]
	\subsubsection{Factor and Reverse Factor Formula}
	\begin{equation*} \begin{gathered}
		sin(A)+sin(B) = 2sin(\tfrac{A+B}{2})cos(\tfrac{A-B}{2}) \\
		sin(A)-sin(B) = 2cos(\tfrac{A+B}{2})sin(\tfrac{A-B}{2}) \\
		cos(A)+cos(B) = 2cos(\tfrac{A+B}{2})cos(\tfrac{A-B}{2}) \\
		cos(A)-cos(B) = -2sin(\tfrac{A+B}{2})sin(\tfrac{A-B}{2}) \\
		sin(A)cos(B) = \tfrac{1}{2} [ sin(A+B) + sin(A-B) ] \\
		cos(A)sin(B) = \tfrac{1}{2} [ sin(A+B) - sin(A-B) ] \\ 
		cos(A)cos(B) = \tfrac{1}{2} [ cos(A+B) + cos(A-B) ] \\
		sin(A)sin(B) = -\tfrac{1}{2} [ cos(A+B) - cos(A-B) ]
	\end{gathered} \end{equation*}

\end{document}